iris/ProofUart.v
@@ -82,8 +82,10 @@ Context `{CID : CpuId}.
   iDestruct (reg_valid_dq with "Hreg Hhtif") as %Lhtif.
   iDestruct (reg_valid_dq with "Hreg Hmisa") as %Lmisa.
   iDestruct "Hdev" as "(Hua & Hpldev & Hvdev)".
-  iInv "Hdinv" as ">Hdbody" "Hdclose".
-  iDestruct "Hdbody" as (u p vst) "(Huf & Hplf & Hvf & Hg & Hlease & %Hpok & %Hvok)".
+  (* only the UART half of the fabric is touched, and [↑uartN ⊆ ↑devN] *)
+  iDestruct (dev_inv_uart with "Hdinv") as "#Huinv".
+  iInv "Huinv" as ">Hdbody" "Hdclose".
+  iDestruct "Hdbody" as (u) "(Huf & Hg)".
   iDestruct (uart_agree with "Hua Huf") as %Hduart.
   destruct (uart_write_total u off storebyte Hoff) as [u' Hwrite_u].
   iMod (reg_update _ nextPC _ (add_vec_int pc (if is_rvc then 2 else 4)) with "Hreg Hnpc") as "[Hreg Hnpc]".
@@ -165,9 +167,8 @@ Context `{CID : CpuId}.
     subst s_x d'. reflexivity. }
   iMod (dev_interp_update_uart σ.(mdev) u u' with "[$Hua $Hpldev $Hvdev] Huf") as "[Hdev' Huf']".
   iMod ("Hacc" $! u u' with "[//] Hg HR") as "[Hg' HS]".
-  iMod ("Hdclose" with "[Huf' Hplf Hvf Hg' Hlease]") as "_".
-  { iNext. iExists u', p, vst. iFrame.
-    iSplitR; [iPureIntro; exact Hpok | iPureIntro; exact Hvok]. }
+  iMod ("Hdclose" with "[Huf' Hg']") as "_".
+  { iNext. iExists u'. iFrame. }
   iModIntro. iExists s_x.
   iSplitR.
   { iPureIntro. rewrite Hpceq. change (if is_rvc then 2%Z else 4%Z) with (if is_rvc then 2 else 4). fold s_pc. exact Hstore. }
@@ -379,8 +380,10 @@ Qed.
   iDestruct (reg_valid_dq with "Hreg Hhtif") as %Lhtif.
   iDestruct (reg_valid_dq with "Hreg Hmisa") as %Lmisa.
   iDestruct "Hdev" as "(Hua & Hpldev & Hvdev)".
-  iInv "Hdinv" as ">Hdbody" "Hdclose".
-  iDestruct "Hdbody" as (u p vst) "(Huf & Hplf & Hvf & Hg & Hlease & %Hpok & %Hvok)".
+  (* only the UART half of the fabric is touched, and [↑uartN ⊆ ↑devN] *)
+  iDestruct (dev_inv_uart with "Hdinv") as "#Huinv".
+  iInv "Huinv" as ">Hdbody" "Hdclose".
+  iDestruct "Hdbody" as (u) "(Huf & Hg)".
   iDestruct (uart_agree with "Hua Huf") as %Hduart.
   destruct (uart_read_total u off Hoff) as (b & u' & Hread_u).
   iMod (reg_update _ nextPC _ (add_vec_int pc (if is_rvc then 2 else 4)) with "Hreg Hnpc") as "[Hreg Hnpc]".
@@ -464,9 +467,8 @@ Qed.
   iMod (reg_update _ (R_bitvector_64 (gpr_of_Z (uint rd))) _ (regval_into_reg (ldval b)) with "Hreg Hrdc") as "[Hreg Hrdc]".
   iDestruct ("Hfins" with "[Hrdc]") as "Hfmap".
   { rewrite (gpr_pt_nz rd _ Hrd). iExact "Hrdc". }
-  iMod ("Hdclose" with "[Huf' Hplf Hvf Hg' Hlease]") as "_".
-  { iNext. iExists u', p, vst. iFrame.
-    iSplitR; [iPureIntro; exact Hpok | iPureIntro; exact Hvok]. }
+  iMod ("Hdclose" with "[Huf' Hg']") as "_".
+  { iNext. iExists u'. iFrame. }
   iModIntro. iExists s_x.
   iSplitR.
   { iPureIntro. rewrite Hpceq. change (if is_rvc then 2%Z else 4%Z) with (if is_rvc then 2 else 4). fold s_pc. exact Hload. }
